Revive the signature for poly1305_blocks

src/crypto/poly1305/x64/X64.Poly1305.Math_i.fst
@@ -5,7 +5,7 @@ open FStar.Tactics.Canon
 open FStar.Math.Lemmas
 open FStar.Math.Lib
 open FStar.Mul
-
+open X64.Semantics_s   // needed for mem
 (*
 open FStar.Mul
 open FStar.UInt
@@ -20,6 +20,23 @@ lemma_BitwiseMul64()
 // these settings make it super slow
 // #reset-options "--z3rlimit_factor 4 --z3rlimit 300 --z3cliopt smt.QI.EAGER_THRESHOLD=100 --z3cliopt smt.CASE_SPLIT=3 --z3cliopt smt.arith.nl=false --max_fuel 0 --max_ifuel 0 --smtencoding.elim_box true --eager_inference --smtencoding.nl_arith_repr wrapped --smtencoding.l_arith_repr native"
 
+
+let rec poly1305_heap_blocks (h:int) (pad:int) (r:int) (m:mem) (i:int) 
+        (k:int{i <= k /\ (k - i) % 16 == 0 /\ (forall (j:int) . i <= j /\ j < k /\ (j - i) % 8 = 0 ==> m `Map.contains` j)}) =
+        admit()
+(*
+    requires i <= k
+    requires (k - i) % 16 == 0
+    requires forall j :: i <= j < k && (j - i) % 8 == 0 ==> j in m
+    decreases k - i
+*)
+(*
+    if i = k then h
+    else
+        let kk = k - 16 in
+        let hh = poly1305_heap_blocks h pad r m i kk in
+        modp((hh + pad + nat64_max * m.[kk + 8] + m.[kk]) * r)
+*)
 
 
 #reset-options "--smtencoding.elim_box true --z3cliopt smt.arith.nl=true"
